For all: let m, n & t be integers.

# a

"If m | n, then m^2 | n^2"

Assume that m | n

Then n = mk for some integer k

n^2 = (mk)^2 = m^2(k^2)

Let j = k^2

Then n^2 = m^2(j)

Therefore m^2 | n^2

# b

"If m | n, then m | (7n^3 + 13n^2 - n)"

Assume that m | n, so that n = mk for some integer k.

Then

```
7n^3 + 13n^2 - n
= 7(mk)^3 + 13(mk)^2 - mk
= 7m^3k^3 + 13m^2k^2 - mk
= m(7m^2k^3 + 13mk^2 - k)
```

Then 7n^3 + 13n^2 - n = mj where j is equal to the integer 7m^2k^3 + 13mk^2 - k

Therefore m | 7n^3 + 13n^2 - n

# c

"If m | n and m | t, then m | (n + t)"

Assume that m | n and m | t so that n = mk and t = mj

n + t = mk + mj = m(k + j)

Knowing that the sum of k and j is just some other integer l, then n + t = ml

Therefore m | (n + t)

# d

"If 3 | 2n then 3 | n"

Assume 3 | 2n

The gcd(3, 2) = 1

Using Bezout's identity, then there exist integers k and l such that 1 = 3k + 2l.

Multiplying both sides by n: n = 3nk + 2nl

Because 3 | 2n, 2n = 3m for some integer m.

Substituting 3m for 2n, then n = 3nk + 3ml = n = 3(nk + ml)

Given that nk + ml are just another integer, then 3 | n
