# a

"If n is a positive integer, then 4 divides 1 + (-1)^n * (2n - 1)"

Case 1: n is even

Assume that n is a positive even integer n = 2k for some integer k.

Because n is even, (-1)^n will equal 1

2n - 1 = 2(2k) - 1 = 4k - 1

Plugging these two back in: 1 + (-1)^n * (2n - 1) = 1 + 1(4k - 1) = 4k

Therefore 4 | 1 + (-1)^n * (2n - 1), in the case that n is even.

Case 2: n is odd

Assume that n is a positive odd integer n = 2k + 1 for some integer k.

Because n is odd (-1)^n will equal -1.

2n - 1 = 2(2k + 1) - 1 = 4k + 2 - 1 = 4k + 1

Plugging these two back in: 1 + (-1)^n * (2n - 1) = 1 - 1(4k + 1) = 1 - 4k - 1 = -4k = 4(-k)

Therefore 4 | 1 + (-1)^n * (2n - 1), in the case that n is odd.


# b

"Every multiple of 4 is equal to 1 + (-1)^n * (2n - 1) for some positive integer n"

Examples:
4     = 1 + (-1)^2 * (2(2) - 1) = 1 + 1(4 - 1)  = 4
8     = 1 + (-1)^4 * (2(4) - 1) = 1 + 1(8 - 1)  = 8
12    = 1 + (-1)^6 * (2(6) - 1) = 1 + 1(12 - 1) = 12
16    = 1 + (-1)^8 * (2(8) - 1) = 1 + 1(16 - 1) = 16

0     = 1 + (-1)^1 * (2(1) - 1) = 1 - (2 - 1)   = 0
-4    = 1 + (-1)^3 * (2(3) - 1) = 1 - (6 - 1)   = -4
-8    = 1 + (-1)^5 * (2(5) - 1) = 1 - (10 - 1)  = -8

Let 4k = 1 + (-1)^n * (2n - 1)

Case 1: k is 0

0 = 1 + (-1)^n * (2n - 1)

Plugging in 1 for n results in 0 = 1 - (2(1) - 1) = 0, which is true.

Case 2: k is positive

The right side of the equation can either be the sum of 1 and a positive odd number,
or the sum of 1 and a negative odd number. If the negative odd number is 1, then the
result will be zero, which is the case covered above. All other negative numbers added
to 1 will result in a negative number, but the assumption is that k is positive, so the
sum must be 1 and a positive odd number.

For the sum to be positive n must be even so that (-1)^n is even.

Therefore 4k = 1 + 1(2n - 1) = 2n, so that n = 2k

Case 3: k is negative

Continuing the logic from case 2, if k is negative then n must be odd.

Then 4k = 1 - 1(2n - 1) = 2 - 2n  = 2(1 - n)

2k = 1 - n

Therefore n = 1 - 2k
