# a

a = 3, b = 13

gcd(3, 13) = 1
gcd(3, 13) = 3(k) + 13(l) = 3(-4) + 13(1) = -12 + 13 = 1
k = -4
l = 1

# b

a = 13, b = 3

gcd(13, 3) = 1
gcd(13, 3) = 13(k) + 3(l) = 13(1) + 3(-4) = 13 - 12 = 1
k = 1
l = -4

# c

a = -25, b = 40
gcd(-25, 40) = 5
gcd(-25, 40) = -25k + 40l = -25(3) + 40(2) = -75 + 80 = 5
k = 3
l = 2

# d

a = -22, b = -14
gcd(-22, -14) = 2
gcd(-22, -14) = -22k + -14l =  -22(5) + 14(-8) = 2

k = 5
l = -8

# e

a = 62
b = 48

gcd(62, 48) = 2
gcd(62, 48) = 62k + 48l = 62(7) + 48(-9) = 2

k = 7
l = -9

# f

a = 13
b = -50
gcd(13, -50) = 1
gcd(13, -50) = 13k + -50l = 13(27) + -50(7) = 1

k = 27
l = 7
