# version 1

## lemma 1

Given positive integers a, b and r:

If:

 b = ak + r, 0 <= r < a
-b = aj + t, 0 <= t < a

Then:

-k - j = 1

PROOF:

aj + t = -ak - r
aj + ak = -t - r
a(j + k) = -t - r
a(j + k) = -(t + r)

Note that because the left side is divisible by a, so is the right side.

0 < t + r < 2a

So t + r is: positive, a multiple of a, and less than 2a. The only multiple of a on that interval is a.

Therefore

a(j + k) = -a
j + k    = -1

1 = -k - j

## main

"If a and b are both positive integers and a divides b with a non-zero remainder of r,
 then a divides -b with a remainder of a - r"

PROOF:

 b = ak + r, 0 < r < a
-b = aj + t, 0 <= t < a

-ak - r = aj + t
t = -ak - aj - r
  = a(-k - j) - r

Using lemma 1, -k - j is equal to 1, so t = a(1) - r = a - r, which is what was sought.

# version 2

"If a and b are both positive integers and a divides b with a non-zero remainder of r,
 then a divides -b with a remainder of a - r"

Let b = ak + r, 0 < r < a

Then

-b = -ak - r
   = -ak - r - a + a
   = -ak - a + a - r
   = a(-k - 1) + (a - r)
