"""
Assume that a, b, c, d and n are integers. Also assume that a ≡ b (mod n) and c ≡ d (mod n).

Prove

(i) a - c ≡ b - d (mod n)
(ii) ac = bd (mod n)
"""

# i

If `a ≡ b (mod n)` then `n | a - b` and therefore `a - b = nk` for some integer k.

Also, if `c ≡ d (mod n)` then `n | c - d` and therefore `c - d = nj` for some integer j.

with some algebra:

```
a - b - c + d = nk - nj
(a - c) - (b - d) = n(k - j)
```

Therefore `n | (a - c) - (b - d)` which means that `a - c ≡ b - d (mod n)`

# ii

If `a ≡ b (mod n)` then `n | a - b` and therefore `a - b = nk` and `a = nk + b`for some integer k.

Also, if `c ≡ d (mod n)` then `n | c - d` and therefore `c - d = nj` and `c = nj + d` for some integer j.

With some algebra:

```
ac = (nk + b)(nj + d) = n^2kj + nkd + bnj + bd = n(nkj + dk + bj) + bd
```

Then

`ac - bd = n(nkj + dk + bj)`

Because `nkj + dk + bj` is also an integer `n | ac - bd` and therefore `ac = bd (mod n)`
