# a

"the sum of an even integer and an odd integer is odd"

2 + 3   = 5
8 + 7   = 15
12 + 11 = 23

Let a be even and b be odd.

a can be rewritten as 2k
b can be rewritten as 2l + 1

Then their sum can be written as (2k) + (2l + 1) = 2(k + l) + 1

By fact 2.1, 2(k + l) + 1 can be considered 2j + 1 for some integer j.

This is the definition of odd.

# b

"the product of two even integers is even"

4 * 2   = 8
8 * 8   = 64
10 * 10 = 100

Let a and b be even.

a can be rewritten as 2k for some integer k
b can be rewritten as 2l for some integer l

Then their sum is 2k + 2l = 2(k + l)

By fact 2.1, 2(k + l) can be considered as 2j for some integer j.

This is the definition of even.

# c

"the product of two odd integers is odd"

3 * 3 = 9
3 * 5 = 15
7 * 9 = 63

Let a & b be odd.

Then a = 2k + 1 for some integer k
and b = 2l + 1 for some integer l

Their product: (2k + 1)(2l + 1) = 4kl + 2k + 2l + 1 = 2(kl + k + l) + 1

By fact 2.1, 2(kl + k + l) can be considered as 2j for some integer j.
Therefore 2(kl + k + l) + 1 can be considered 2j + 1.

This is the definition of odd.

# d

"the product of an even integer and an odd integer is even"

3 * 4 = 12
5 * 6 = 30
7 * 8 = 56

Let a be even and b be odd.

Then a = 2k for some integer k
and b = 2l + 1 for some integer l.

Their product: 2k * (2l + 1) = 2kl + 2k = 2(kl + K)

By fact 2.1, 2(kl + k) can be considered 2j for some integer j.

This is the definition of even.

# e

"an even integer squared is an even integer"

2^2 = 4
4^2 = 16
6^2 = 36

Let n be even.

Then n^2 is the same thing as n * n, which is an even number multiplied by an even number.

By proof "#B" this is true.

For exercise though:

n can be written as 2k. So n^2 is 2k(2k) = 4k^2 = 2(2k^2).

By fact 2.1, 2(2k^2) can be considered 2j for some integer j.

This is the definition of even.
