# a

"If n is an even integer, then -n is an even integer"

Examples:
4 & -4
2 & -2
8 & -8

Let n be an even integer.

So n = 2k for some integer k.

Then -n = 2(-1)(k)

We can write this as 2j for the integer that represents (-1)(k).

This is the definition of an even integer.

# b

"If n is an odd integer, then -n is an odd integer"

Examples:
3 & -3
5 & -5
7 & -7

Let n be an odd integer

Then n = (2k + 1) for some integer k

-n = -1(2k + 1)
   = -2k - 1
   = -2k - 1 + 1 - 1
   = -2k - 2 + 1
   = 2(-k - 1) + 1
   = 2j + 1 where j = -k - 1

2j + 1 is the definition of odd.

# c

"If n is an even integer, then (-1)^n = 1"

Examples:
(-1)^2 = (-1)(-1) = 1
(-1)^4 = (-1)(-1)(-1)(-1) = 1
(-1)^6 = (-1)(-1)(-1)(-1)(-1)(-1) = 1

Let n be even, so that n = 2k for some integer k

Then (-1)^2k = ((-1)^2)^k = 1^k = 1
