# a

"If n is odd, then n^2 + 4n + 9 is even"

Let n be odd. Then n = 2k + 1 for some integer k.

= (2k + 1)^2 + 4(2k + 1) + 9
= 4k^2 + 4k + 1 + 8k + 4 + 9
= 4k^2 + 12k + 10
= 2(2k^2 + 6k + 5)
= 2j

where j = 2k^2 + 6k + 5

2j is the definition of an even number.

# b

"If n is odd, then n^3 is odd"

Let n be odd. Then n = 2k + 1 for some integer k.

n^3
= (2k + 1)^3
= 8k^3 + 12k^2 + 6k + 1
= 2(4k^3 + 6k^2 + 3k) + 1
= 2j + 1

where j = 4k^3 + 6k^2 + 3k

2j + 1 is the definition for an odd number.


# c

"If n is even, then n + 1 is odd"

Let n be even. Then n = 2k for some integer k

n + 1 = 2k + 1, which is the definition of an odd number.
