# a

"If n is an integer, then n^2 + n is even"

2^2 + 2 = 6, even
3^3 + 3 = 12, even
5^2 + 5 = 30, even

case 1: n is even

If n is even then it can be written as 2k for some integer k.

n^2 + n = (2k)^2 + 2k = 4k^2 + 2k = 2(2k^2 + k)

Using Fact 2.1 this number is even.

Case 2: n is odd.

If n is odd, then it can be written as 2k + 1 for some integer k.

n^2 + n = (2k + 1)^2 + (2k + 1) = 4k^2 + 4k + 1 + 2k + 1 = 4k^2 + 6k + 2 = 2(2k^2 + 3k + 1)

Using Fact 2.1 this number is even.

# b

"If n is an integer, 3n^2 + 5n + 1 is odd"

3(2)^2 + 5(2) + 1 = 23, odd
3(3)^2 + 5(3) + 1 = 43, odd

Case 1: n is even

If n is even then it can be written as 2k for some integer k.

3n^2 + 5n + 1 = 3(2k)^2 + 5(2k) + 1 = 12k^2 + 10k + 1 = 2(6k^2 + 5k) + 1

By fact 2.1, this number is odd.

Case 2: n is odd

If n is odd, then it can be written as 2k + 1 for some integer k.

3n^2 + 5n + 1 = 3(2k + 1)^2 + 5(2k + 1) + 1 = 12k^2 + 22k + 8 + 1 = 2(6k^2 + 11k + 4) + 1

Using Fact 2.1, this number is odd.

# c

"If n is an integer, then n^2 + 3n - 6 is even"

(2)^2 + 3(2) - 6 = 4, even
(3)^2 + 3(3) - 6 = 12, even

Case 1: n is even

Let n = 2k for some integer k

n^2 + 3n - 6 = (2k)^2 + 3(3k) - 6 = 4k^2 + 12k - 6 = 2(2k^2 + 6k - 3)

By fact 2.1, even.

Case 2: n is odd

Let n = 2k + 1 for some integer k

n^2 + 3n - 6 = (2k + 1)^2 + 3(2k + 1) - 6 = 4k^2 + 10k + 4 = 2(2k^2 + 5k + 2)

By face 2.1, even.

# d

"If m & n are integers of the same parity, 7m - 3n is even"

Case 1: m & n are both even.

Let m = 2k for some integer k
and n = 2j for some integer j

7m - 3n = 7(2k) + 3(2j) = 2(7k + 3j)

By fact 2.1, this number is even.

Case 2: m & n are both odd

Let m = 2k + 1 for some integer k
and n = 2j + 1 for some integer j

7m - 3n = 7(2k + 1) - 3(2k + 1) = 14k + 7 - 6k - 3 = 20k + 4 = 2(10k + 2)

By fact 2.1, this number is even.
